src/ModAdequacy.v
@@ -1,0 +1,60 @@
+From sflib Require Import sflib.
+From ITree Require Export ITree.
+From Paco Require Import paco.
+
+Require Export Coq.Strings.String.
+Require Import Program.
+
+From ExtLib Require Import FMapAList.
+
+Export ITreeNotations.
+
+From Fairness Require Import pind8.
+From Fairness Require Export ITreeLib FairBeh FairSim.
+From Fairness Require Export Mod ModSimPico Concurrency.
+
+Set Implicit Arguments.
+
+
+
+Section ADEQ.
+
+  Variable state_src: Type.
+  Variable state_tgt: Type.
+
+  Variable _ident_src: ID.
+  Definition ident_src := id_sum tids _ident_src.
+  Variable _ident_tgt: ID.
+  Definition ident_tgt := id_sum tids _ident_tgt.
+
+  Variable wf_src: WF.
+  Variable wf_tgt: WF.
+
+  Let srcE := ((@eventE ident_src +' cE) +' sE state_src).
+  Let tgtE := ((@eventE ident_tgt +' cE) +' sE state_tgt).
+
+  Variable world: Type.
+  Variable world_le: world -> world -> Prop.
+
+  Variable I: (@shared state_src state_tgt ident_src ident_tgt wf_src wf_tgt world) -> Prop.
+
+  Theorem local_adequacy
+          R
+          (ths_src: @threads _ident_src (sE state_src) R)
+          (ths_tgt: @threads _ident_tgt (sE state_tgt) R)
+          (LSIM: forall tid0 (src0: itree srcE R) (tgt0: itree tgtE R)
+                   (LSRC: Some src0 = threads_find tid0 ths_src)
+                   (LTGT: Some tgt0 = threads_find tid0 ths_tgt),
+              local_sim world_le I src0 tgt0)
+          tid src tgt (st_src: state_src) (st_tgt: state_tgt)
+          (SRC: Some src = threads_find tid ths_src)
+          (TGT: Some tgt = threads_find tid ths_tgt)
+    :
+    gsim wf_src wf_tgt (@eq R) false false
+         (interp_all st_src ths_src tid src)
+         (interp_all st_tgt ths_tgt tid tgt).
+  Proof.
+
+  Abort.
+
+End ADEQ.
